mostly some miscellaneous things

Picinae_riscv.v
@@ -173,7 +173,7 @@ Definition rv_decode_binop n :=
   end.
 
 Definition rv_decode_branch n :=
-  match N.lor (xbits n 12 15) (N.land n 256) with 
+  match N.lor (xbits n 12 15) (N.land n 256) with
   | 0 => R5_Beq | 1 => R5_Bne | 4 => R5_Blt | 5 => R5_Bge | 6 => R5_Bltu | 7 => R5_Bgeu
   | _ => (fun _ _ _ => R5_InvalidI)
   end.
@@ -209,23 +209,23 @@ Definition rv_decode_op op n :=
     end
   | 23 => R5_Auipc (xbits n 7 12) (N.land n (N.shiftl (N.ones 20) 12))
   | 35 => rv_decode_store n (xbits n 15 20) (xbits n 20 25)
-            (toZ 12 (N.lor (N.shiftl (xbits n 25 32) 5) (xbits n 7 12)))
+                          (toZ 12 (N.lor (N.shiftl (xbits n 25 32) 5) (xbits n 7 12)))
   | 51 => rv_decode_binop n (xbits n 7 12) (xbits n 15 20) (xbits n 20 25)
   | 55 => R5_Lui (xbits n 7 12) (N.land n (N.shiftl (N.ones 20) 12))
   | 99 => rv_decode_branch n (xbits n 15 20) (xbits n 20 25)
-            (toZ 13 (N.lor (N.shiftl (xbits n 8 12) 1)
-                      (N.lor (N.shiftl (xbits n 25 31) 5)
-                        (N.lor (N.shiftl (xbits n 7 8) 11)
-                          (N.shiftl (xbits n 31 32) 12)))))
+                           (toZ 13 (N.lor (N.shiftl (xbits n 8 12) 1)
+                                          (N.lor (N.shiftl (xbits n 25 31) 5)
+                                                 (N.lor (N.shiftl (xbits n 7 8) 11)
+                                                        (N.shiftl (xbits n 31 32) 12)))))
   | 103 => match xbits n 12 15 with
            | 0 => R5_Jalr (xbits n 7 12) (xbits n 15 20) (toZ 12 (xbits n 20 32))
            | _ => R5_InvalidI
            end
   | 111 => match xbits n 21 22 with
            | 0 => R5_Jal (xbits n 7 12) (toZ 21 (N.lor (N.shiftl (xbits n 21 31) 1)
-                                           (N.lor (N.shiftl (xbits n 20 21) 11)
-                                             (N.lor (N.shiftl (xbits n 12 20) 12)
-                                               (N.shiftl (xbits n 31 32) 20)))))
+                                                       (N.lor (N.shiftl (xbits n 20 21) 11)
+                                                              (N.lor (N.shiftl (xbits n 12 20) 12)
+                                                                     (N.shiftl (xbits n 31 32) 20)))))
            | _ => R5_InvalidI
            end
   | _ => R5_InvalidI
@@ -322,74 +322,74 @@ Definition rv_prog : program :=
 
 Lemma hastyp_r5mov:
   forall c0 c n e (TS: hastyp_stmt c0 c (Move (rv_varid n) e) c),
-  hastyp_stmt c0 c (r5mov n e) c.
+    hastyp_stmt c0 c (r5mov n e) c.
 Proof.
   intros. destruct n. apply TNop. exact TS.
 Qed.
 
 Lemma hastyp_rvmov:
   forall n e (TE: hastyp_exp rvtypctx e (NumT 32)),
-  hastyp_stmt rvtypctx rvtypctx (Move (rv_varid n) e) rvtypctx.
+    hastyp_stmt rvtypctx rvtypctx (Move (rv_varid n) e) rvtypctx.
 Proof.
   intros. erewrite store_upd_eq at 3.
-    apply TMove.
-      right. destruct n as [|n]. reflexivity. repeat first [ reflexivity | destruct n as [n|n|] ].
-      exact TE.
-    destruct n as [|n]. reflexivity. repeat first [ reflexivity | destruct n as [n|n|] ].
+  apply TMove.
+  right. destruct n as [|n]. reflexivity. repeat first [ reflexivity | destruct n as [n|n|] ].
+  exact TE.
+  destruct n as [|n]. reflexivity. repeat first [ reflexivity | destruct n as [n|n|] ].
 Qed.
 
 Lemma hastyp_r5store:
   forall e (TE: hastyp_exp rvtypctx e (MemT 32)),
-  hastyp_stmt rvtypctx rvtypctx (Move V_MEM32 e) rvtypctx.
+    hastyp_stmt rvtypctx rvtypctx (Move V_MEM32 e) rvtypctx.
 Proof.
   intros. erewrite store_upd_eq at 3.
-    apply TMove.
-      right. reflexivity.
-      exact TE.
-    reflexivity.
+  apply TMove.
+  right. reflexivity.
+  exact TE.
+  reflexivity.
 Qed.
 
 Lemma hastyp_r5var:
   forall n, hastyp_exp rvtypctx (r5var n) (NumT 32).
 Proof.
   intro. destruct n as [|n].
-    apply TWord. reflexivity.
-    apply TVar. repeat first [ reflexivity | destruct n as [n|n|] ].
+  apply TWord. reflexivity.
+  apply TVar. repeat first [ reflexivity | destruct n as [n|n|] ].
 Qed.
 
 Lemma xbits_bound:
   forall n i j w, j-i <= w -> xbits n i j < 2^w.
 Proof.
   intros. unfold xbits. eapply N.lt_le_trans.
-    rewrite N.land_ones. apply N.mod_upper_bound, N.pow_nonzero. discriminate 1.
-    apply N.pow_le_mono_r. discriminate 1. assumption.
+  rewrite N.land_ones. apply N.mod_upper_bound, N.pow_nonzero. discriminate 1.
+  apply N.pow_le_mono_r. discriminate 1. assumption.
 Qed.
 
 Theorem welltyped_rv2il:
   forall a n, hastyp_stmt rvtypctx rvtypctx (rv2il a (rv_decode n)) rvtypctx.
 Proof.
   intros. unfold rv_decode, rv_decode_op, rv_decode_load, rv_decode_store,
-                 rv_decode_binop, rv_decode_branch.
+          rv_decode_binop, rv_decode_branch.
 
   repeat match goal with |- context [ match ?x with _ => _ end ] =>
-    let op := fresh "op" in
-    generalize x; intro op;
-    first [ destruct op as [|op] | destruct op as [op|op|] ];
-    try apply TExn
-  end.
+                         let op := fresh "op" in
+                         generalize x; intro op;
+                           first [ destruct op as [|op] | destruct op as [op|op|] ];
+                           try apply TExn
+         end.
 
   all: repeat first
-  [ reflexivity
-  | discriminate 1
-  | apply hastyp_r5mov
-  | apply hastyp_rvmov
-  | apply hastyp_r5var
-  | apply hastyp_r5store
-  | apply TBinOp with (w:=32)
-  | apply xbits_bound
-  | apply ofZ_bound
-  | apply N.mod_lt
-  | econstructor ].
+              [ reflexivity
+              | discriminate 1
+              | apply hastyp_r5mov
+              | apply hastyp_rvmov
+              | apply hastyp_r5var
+              | apply hastyp_r5store
+              | apply TBinOp with (w:=32)
+              | apply xbits_bound
+              | apply ofZ_bound
+              | apply N.mod_lt
+              | econstructor ].
 
   rewrite N.land_comm. eapply land_bound, N.lt_le_trans. apply shiftl_bound, ones_bound. reflexivity.
 Qed.
@@ -400,8 +400,8 @@ Proof.
   intros s a. unfold rv_prog.
   destruct (s V_MEM32), (s A_EXEC); try exact I.
   destruct (m0 a).
-    exact I.
-    exists rvtypctx. apply welltyped_rv2il.
+  exact I.
+  exists rvtypctx. apply welltyped_rv2il.
 Qed.
 
 
@@ -409,7 +409,7 @@ Qed.
 
 Lemma memacc_read_frame:
   forall h s v u (NE: v <> A_READ),
-  MemAcc mem_readable h (update s v u) = MemAcc mem_readable h s.
+    MemAcc mem_readable h (update s v u) = MemAcc mem_readable h s.
 Proof.
   intros. unfold MemAcc, mem_readable. rewrite update_frame. reflexivity.
   apply not_eq_sym. exact NE.
@@ -417,7 +417,7 @@ Qed.
 
 Lemma memacc_write_frame:
   forall h s v u (NE: v <> A_WRITE),
-  MemAcc mem_writable h (update s v u) = MemAcc mem_writable h s.
+    MemAcc mem_writable h (update s v u) = MemAcc mem_writable h s.
 Proof.
   intros. unfold MemAcc, mem_writable. rewrite update_frame. reflexivity.
   apply not_eq_sym. exact NE.
@@ -425,16 +425,16 @@ Qed.
 
 Lemma memacc_read_updated:
   forall h s v u1 u2,
-  MemAcc mem_readable h (update (update s v u2) A_READ u1) =
-  MemAcc mem_readable h (update s A_READ u1).
+    MemAcc mem_readable h (update (update s v u2) A_READ u1) =
+    MemAcc mem_readable h (update s A_READ u1).
 Proof.
   intros. unfold MemAcc, mem_readable. rewrite !update_updated. reflexivity.
 Qed.
 
 Lemma memacc_write_updated:
   forall h s v u1 u2,
-  MemAcc mem_writable h (update (update s v u2) A_WRITE u1) =
-  MemAcc mem_writable h (update s A_WRITE u1).
+    MemAcc mem_writable h (update (update s v u2) A_WRITE u1) =
+    MemAcc mem_writable h (update s A_WRITE u1).
 Proof.
   intros. unfold MemAcc, mem_writable. rewrite !update_updated. reflexivity.
 Qed.
@@ -462,11 +462,11 @@ Qed.
 (* Simplify memory access assertions produced by step_stmt. *)
 Ltac simpl_memaccs H :=
   try lazymatch type of H with context [ MemAcc mem_writable ] =>
-    rewrite ?memacc_write_frame, ?memacc_write_updated in H by discriminate 1
-  end;
+                               rewrite ?memacc_write_frame, ?memacc_write_updated in H by discriminate 1
+      end;
   try lazymatch type of H with context [ MemAcc mem_readable ] =>
-    rewrite ?memacc_read_frame, ?memacc_read_updated in H by discriminate 1
-  end.
+                               rewrite ?memacc_read_frame, ?memacc_read_updated in H by discriminate 1
+      end.
 
 (* Symbolically evaluate a RISC-V machine instruction for one step. *)
 Ltac rv_step_and_simplify XS :=
@@ -478,7 +478,7 @@ Ltac rv_step_and_simplify XS :=
 (* Some versions of Coq check injection-heavy proofs very slowly (at Qed).  This slow-down can
    be avoided by sequestering prevalent injections into lemmas, as we do here. *)
 Remark inj_prog_stmt: forall (sz1 sz2: N) (q1 q2: stmt),
-                      Some (sz1,q1) = Some (sz2,q2) -> sz1=sz2 /\ q1=q2.
+    Some (sz1,q1) = Some (sz2,q2) -> sz1=sz2 /\ q1=q2.
 Proof. injection 1 as. split; assumption. Qed.
 
 (* Simplify (exitof a x) without expanding a. *)
@@ -494,7 +494,7 @@ Remark exitof_some a x: exitof a (Some x) = x. Proof eq_refl.
    to be solved manually by the user. *)
 Ltac prove_prog_exits :=
   solve [ reflexivity | assumption |
-    match goal with [ H: forall s, ?p s ?a = None |- ?p _ ?a = None ] => apply H end ].
+          match goal with [ H: forall s, ?p s ?a = None |- ?p _ ?a = None ] => apply H end ].
 
 (* If asked to step the computation when we're already at an invariant point,
    just make the proof goal be the invariant. *)
@@ -511,23 +511,23 @@ Ltac rv_invhere :=
 Ltac rv_invseek :=
   apply NIStep; [reflexivity|];
   let sz := fresh "sz" in let q := fresh "q" in let s := fresh "s" in let x := fresh "x" in
-  let IL := fresh "IL" in let XS := fresh "XS" in
-  intros sz q s x IL XS;
-  apply inj_prog_stmt in IL; destruct IL; subst sz q;
-  rv_step_and_simplify XS;
-  repeat lazymatch type of XS with
-         | s=_ /\ x=_ => destruct XS; subst s x
-         | exec_stmt _ _ (if ?c then _ else _) _ _ =>
-             let BC := fresh "BC" in destruct c eqn:BC;
-             rv_step_and_simplify XS
-         | exec_stmt _ _ (N.iter _ _ _) _ _ => fail
-         | _ => rv_step_and_simplify XS
-         end;
-  repeat match goal with [ u:value |- _ ] => clear u
-                       | [ n:N |- _ ] => clear n
-                       | [ m:addr->N |- _ ] => clear m end;
-  try lazymatch goal with |- context [ exitof (N.add ?m ?n) ] => simpl (N.add m n) end;
-  try first [ rewrite exitof_none | rewrite exitof_some ].
+                                                                      let IL := fresh "IL" in let XS := fresh "XS" in
+                                                                                              intros sz q s x IL XS;
+                                                                                              apply inj_prog_stmt in IL; destruct IL; subst sz q;
+                                                                                              rv_step_and_simplify XS;
+                                                                                              repeat lazymatch type of XS with
+                                                                                                     | s=_ /\ x=_ => destruct XS; subst s x
+                                                                                                     | exec_stmt _ _ (if ?c then _ else _) _ _ =>
+                                                                                                       let BC := fresh "BC" in destruct c eqn:BC;
+                                                                                                                               rv_step_and_simplify XS
+                                                                                                     | exec_stmt _ _ (N.iter _ _ _) _ _ => fail
+                                                                                                     | _ => rv_step_and_simplify XS
+                                                                                                     end;
+                                                                                              repeat match goal with [ u:value |- _ ] => clear u
+                                                                                                                | [ n:N |- _ ] => clear n
+                                                                                                                | [ m:addr->N |- _ ] => clear m end;
+                                                                                              try lazymatch goal with |- context [ exitof (N.add ?m ?n) ] => simpl (N.add m n) end;
+                                                                                              try first [ rewrite exitof_none | rewrite exitof_some ].
 
 (* Clear any stale memory-access hypotheses (arising from previous computation
    steps) and either step to the next machine instruction (if we're not at an
@@ -539,74 +539,25 @@ Ltac rv_step :=
 
 Module RISCVNotations.
 
-Notation "Ⓜ m" := (VaM m 32) (at level 20). (* memory value *)
-Notation "ⓑ u" := (VaN u 1) (at level 20). (* bit value *)
-Notation "Ⓑ u" := (VaN u 8) (at level 20). (* byte value *)
-Notation "Ⓦ u" := (VaN u 16) (at level 20). (* word value *)
-Notation "Ⓓ u" := (VaN u 32) (at level 20). (* dword value *)
-Notation "m Ⓑ[ a  ]" := (getmem LittleE 1 m a) (at level 10). (* read byte from memory *)
-Notation "m Ⓦ[ a  ]" := (getmem LittleE 2 m a) (at level 10). (* read word from memory *)
-Notation "m Ⓓ[ a  ]" := (getmem LittleE 4 m a) (at level 10). (* read dword from memory *)
-Notation "m [Ⓑ a := v  ]" := (setmem LittleE 1 m a v) (at level 50, left associativity). (* write byte to memory *)
-Notation "m [Ⓦ a := v  ]" := (setmem LittleE 2 m a v) (at level 50, left associativity). (* write word to memory *)
-Notation "m [Ⓓ a := v  ]" := (setmem LittleE 4 m a v) (at level 50, left associativity). (* write dword to memory *)
-Notation "x ⊕ y" := ((x+y) mod 2^32) (at level 50, left associativity). (* modular addition *)
-Notation "x ⊖ y" := ((x-y) mod 2^32) (at level 50, left associativity). (* modular subtraction *)
-Notation "x ⊗ y" := ((x*y) mod 2^32) (at level 40, left associativity). (* modular multiplication *)
-Notation "x << y" := (N.shiftl x y) (at level 40, left associativity). (* logical shift-left *)
-Notation "x >> y" := (N.shiftr x y) (at level 40, left associativity). (* logical shift-right *)
-Notation "x >>> y" := (ashiftr 32 x y) (at level 40, left associativity). (* arithmetic shift-right *)
-Notation "x .& y" := (N.land x y) (at level 25, left associativity). (* logical and *)
-Notation "x .^ y" := (N.lxor x y) (at level 25, left associativity). (* logical xor *)
-Notation "x .| y" := (N.lor x y) (at level 25, left associativity). (* logical or *)
+  Notation "Ⓜ m" := (VaM m 32) (at level 20). (* memory value *)
+  Notation "ⓑ u" := (VaN u 1) (at level 20). (* bit value *)
+  Notation "Ⓑ u" := (VaN u 8) (at level 20). (* byte value *)
+  Notation "Ⓦ u" := (VaN u 16) (at level 20). (* word value *)
+  Notation "Ⓓ u" := (VaN u 32) (at level 20). (* dword value *)
+  Notation "m Ⓑ[ a  ]" := (getmem LittleE 1 m a) (at level 10). (* read byte from memory *)
+  Notation "m Ⓦ[ a  ]" := (getmem LittleE 2 m a) (at level 10). (* read word from memory *)
+  Notation "m Ⓓ[ a  ]" := (getmem LittleE 4 m a) (at level 10). (* read dword from memory *)
+  Notation "m [Ⓑ a := v  ]" := (setmem LittleE 1 m a v) (at level 50, left associativity). (* write byte to memory *)
+  Notation "m [Ⓦ a := v  ]" := (setmem LittleE 2 m a v) (at level 50, left associativity). (* write word to memory *)
+  Notation "m [Ⓓ a := v  ]" := (setmem LittleE 4 m a v) (at level 50, left associativity). (* write dword to memory *)
+  Notation "x ⊕ y" := ((x+y) mod 2^32) (at level 50, left associativity). (* modular addition *)
+  Notation "x ⊖ y" := ((x-y) mod 2^32) (at level 50, left associativity). (* modular subtraction *)
+  Notation "x ⊗ y" := ((x*y) mod 2^32) (at level 40, left associativity). (* modular multiplication *)
+  Notation "x << y" := (N.shiftl x y) (at level 40, left associativity). (* logical shift-left *)
+  Notation "x >> y" := (N.shiftr x y) (at level 40, left associativity). (* logical shift-right *)
+  Notation "x >>> y" := (ashiftr 32 x y) (at level 40, left associativity). (* arithmetic shift-right *)
+  Notation "x .& y" := (N.land x y) (at level 25, left associativity). (* logical and *)
+  Notation "x .^ y" := (N.lxor x y) (at level 25, left associativity). (* logical xor *)
+  Notation "x .| y" := (N.lor x y) (at level 25, left associativity). (* logical or *)
 
 End RISCVNotations.
-
-Inductive rv_encode_type : Set :=
-  | R5ER | R5EI | R5ES | R5EU.
-
-Print rv_asm.
-
-Definition rv_type :=
-  | R5_Lb : N -> N -> N -> rv_asm
-  | R5_Lh : N -> N -> N -> rv_asm
-  | R5_Lw : N -> N -> N -> rv_asm
-  | R5_Lbu : N -> N -> N -> rv_asm
-  | R5_Lhu : N -> N -> N -> rv_asm
-  | R5_Auipc : N -> N -> rv_asm
-  | R5_Sb : N -> N -> Z -> rv_asm
-  | R5_Sh : N -> N -> Z -> rv_asm
-  | R5_Sw : N -> N -> Z -> rv_asm
-  | R5_Add : N -> N -> N -> rv_asm
-  | R5_Sub : N -> N -> N -> rv_asm
-  | R5_Sll : N -> N -> N -> rv_asm
-  | R5_Slt : N -> N -> N -> rv_asm
-  | R5_Sltu : N -> N -> N -> rv_asm
-  | R5_Xor : N -> N -> N -> rv_asm
-  | R5_Srl : N -> N -> N -> rv_asm
-  | R5_Sra : N -> N -> N -> rv_asm
-  | R5_Or : N -> N -> N -> rv_asm
-  | R5_And : N -> N -> N -> rv_asm
-  | R5_Lui : N -> N -> rv_asm
-  | R5_Beq : N -> N -> Z -> rv_asm
-  | R5_Bne : N -> N -> Z -> rv_asm
-  | R5_Blt : N -> N -> Z -> rv_asm
-  | R5_Bge : N -> N -> Z -> rv_asm
-  | R5_Bltu : N -> N -> Z -> rv_asm
-  | R5_Bgeu : N -> N -> Z -> rv_asm
-  | R5_Jalr : N -> N -> Z -> rv_asm
-  | R5_Jal : N -> Z -> rv_asm
-  | R5_Addi : N -> N -> N -> rv_asm
-  | R5_Slli : N -> N -> N -> rv_asm
-  | R5_Slti : N -> N -> N -> rv_asm
-  | R5_Sltiu : N -> N -> N -> rv_asm
-  | R5_Xori : N -> N -> N -> rv_asm
-  | R5_Ori : N -> N -> N -> rv_asm
-  | R5_Andi : N -> N -> N -> rv_asm
-  | R5_Srli : N -> N -> N -> rv_asm
-  | R5_Srai : N -> N -> N -> rv_asm
-  | R5_Fence : N -> N -> rv_asm
-  | R5_Fence_i : rv_asm
-  | R5_InvalidI : rv_asm
-
-Definition rv_encode :=
