Picinae_riscv_encode.v
@@ -1,0 +1,273 @@
+Require Import Coq.Lists.List.
+
+Import ListNotations.
+Import RISCVNotations.
+
+(* Definition list2bv' : list (N * N) -> N * N := *)
+(*   fold_right *)
+(*     (fun (kar kdr : N*N) => *)
+(*        let (len,obj) := kar in let (tlen,tobj) := kdr in *)
+(*        (len + tlen, obj << tlen .| tobj)) *)
+(*     (0,0). *)
+
+Fixpoint list2bv (l : list (N * N)) : N * N :=
+  match l with
+  | [] => (0,0)
+  | (len,obj)::t =>
+    let (tlen,tobj) := list2bv t in
+    (len + tlen, (obj << tlen) .| tobj)
+  end.
+
+Theorem list2bv_len l :
+  fst (list2bv l) = fold_right N.add 0 (map fst l).
+  induction l; auto.
+  simpl.
+  destruct a,list2bv.
+  simpl in *.
+  subst.
+  reflexivity.
+Qed.
+
+Definition bv_valid (bv : N * N) : Prop :=
+  snd bv < 2^(fst bv).
+
+Definition bvl_valid bvl : Prop :=
+  Forall bv_valid bvl.
+
+Theorem list2bv_num l :
+  bvl_valid l -> bv_valid (list2bv l).
+  unfold bvl_valid,bv_valid.
+  induction l; simpl; [reflexivity|].
+  intros.
+  inversion H; subst.
+  destruct a,list2bv.
+  apply concat_bound; tauto.
+Qed.
+
+(*
+  RV32I defines "base instruction formats" R, I, S and U as well as "immediate
+  encoding variants" B and J. B is a variant of S and J is a variant of U.
+  The U base instruction format is special in that it does not directly take an
+  immediate but implicitly shifts the bits of the immediate by 12 so that they
+  form the leading bits of a 32-bit immediate.
+ *)
+Definition rv_encodel_r (opcode funct rd rs1 rs2 : N) :=
+  [(7,funct >> 3);(5,rs2);(5,rs1);(3,xbits funct 0 3);(5,rd);(7,opcode)].
+Definition rv_encodel_i (opcode funct rd rs1 imm : N) :=
+  [(12,imm);(5,rs1);(3,funct);(5,rd);(7,opcode)].
+Definition rv_encodel_s (opcode funct rs1 rs2 imm : N) :=
+  [(7,imm >> 5);(5,rs2);(5,rs1);(3,funct);(5,xbits imm 0 5);(7,opcode)].
+Definition rv_encodel_u_raw (opcode rd immbits : N) :=
+  [(20,immbits);(5,rd);(7,opcode)].
+Definition rv_encodel_u_opt (opcode rd imm : N) :=
+  if xbits imm 0 12 == 0
+  then Some (rv_encodel_u_raw opcode rd (imm >> 12))
+  else None.
+
+(*
+  The B instruction format variant sacrifices the least significant bit of the
+  immediate in the S instruction format to encode 13-bit even immediates. These
+  represent 2-byte-aligned (16-bit-aligned) instruction offsets.
+
+  The variant looks unusual but is sensible when implemented in hardware: the
+  MSB of the B immediate takes the place of the MSB of the S immediate. The
+  positions of the middle bits of the S immediate remain the same, and the bit
+  in the position that originally represented the LSB of the S immediate is
+  replaced by its MSB in the B variant:
+
+   S-immediate: 11,10, 9, 8, 7, 6, 5, 4, 3, 2, 1, 0
+   B-immediate: 12,10, 9, 8, 7, 6, 5, 4, 3, 2, 1,11
+
+  Keeping the MSBs in the same position simplifies sign-extension.
+ *)
+Definition rv_encode_bimm2simm bimm :=
+  if xbits bimm 0 1 == 0
+  then Some (list2bv [(1,bimm >> 12);(10,xbits bimm 1 11);(1,xbits bimm 11 12)])
+  else None.
+Definition rv_encodel_b_opt opcode funct rs1 rs2 imm :=
+  match rv_encode_bimm2simm imm with
+  | None => None
+  | Some simm => Some (rv_encodel_s opcode funct rs1 rs2 (snd simm))
+  end.
+
+(*
+  The J immediate variant is even weirder than the B immediate variant. It only
+  makes sense when compared with the rest of the instruction formats/variants:
+
+   R-immediate:
+   I-immediate: 11,10, 9, 8, 7, 6, 5, 4, 3, 2, 1, 0
+   S-immediate: 11,10, 9, 8, 7, 6, 5, 4, 3, 2, 1, 0
+   B-immediate: 12,10, 9, 8, 7, 6, 5, 4, 3, 2, 1,11
+   U-immediate: 31,30,29,28,27,26,25,24,23,22,21,20,19,18,17,16,15,14,13,12
+   J-immediate: 20,10, 9, 8, 7, 6, 5, 4, 3, 2, 1,11,19,18,17,16,15,14,13,12
+
+  The locations of bits 1-11 are borrowed from B (itself borrowing 1-10 from I
+  and S). The locations of bits 12-19 are borrowed from U. Bit 20 is the MSB,
+  which is the very first bit of any immediate format. Bits 21-31 are
+  sign-extended and bit 0 is implicitly zero (same as with B immediates).
+ *)
+Definition rv_encodel_jimm jimm :=
+  if xbits jimm 0 1 == 0
+  then Some
+         (list2bv
+            [(1,jimm >> 20);(10,xbits jimm 1 11);(1,xbits jimm 11 2)
+             ;(8,xbits jimm 12 20)])
+  else None.
+Definition rv_encodel_j_opt (opcode rd imm : N) :=
+  match rv_encodel_jimm imm with
+  | None => None
+  | Some immbits => Some (rv_encodel_u_raw opcode rd (snd immbits))
+  end.
+
+Print rv_asm.
+Search "decidable".
+
+Definition bvl_valid_dec bvl : {bvl_valid bvl} + {~bvl_valid bvl}.
+  apply Forall_dec.
+  unfold bv_valid,N.lt.
+  intros.
+  destruct (_ ?= _); [|left;reflexivity|]; right; discriminate.
+Qed.
+
+Definition list2bv_opt bvl :=
+  if bvl_valid_dec bvl then Some (list2bv bvl) else None.
+
+Definition rv_encode_r opcode funct rd rs1 rs2 :=
+  list2bv_opt (rv_encodel_r opcode funct rd rs1 rs2).
+Definition rv_encode_i opcode funct rd rs1 imm :=
+  list2bv_opt (rv_encodel_i opcode funct rd rs1 imm).
+Definition rv_encode_s opcode funct rs1 rs2 imm :=
+  list2bv_opt (rv_encodel_s opcode funct rs1 rs2 imm).
+
+Fixpoint encode_le_bits (l : list N) :=
+  match l with
+  | x::xs => x + (encode_le_bits xs << 1)
+  | [] => 0
+  end.
+
+Definition encode_be_bits l :=
+  encode_le_bits (rev l).
+
+Definition rv_encode_addi :=
+  rv_encode_i (encode_be_bits [0;0;1;0;0;1;1]) (encode_be_bits [0;0;0]).
+
+Search "rv" "decode".
+
+Theorem ones_alt_decomp n : N.ones (N.succ n) = N.succ (N.double (N.ones n)).
+  unfold N.ones.
+  destruct n; auto.
+  simpl.
+  rewrite Pos.iter_succ.
+  simpl.
+  destruct p using Pos.peano_ind; auto.
+  rewrite Pos.iter_succ.
+  reflexivity.
+Qed.
+
+Theorem rv_shift_and_ones x shl one :
+  one <= shl -> (x << shl) .& N.ones one = 0.
+  rewrite N.land_ones.
+  rewrite N.shiftl_mul_pow2.
+  intros.
+  rewrite <- (N.sub_add one shl) by assumption.
+  rewrite N.pow_add_r.
+  rewrite N.mul_assoc.
+  rewrite N.mod_mul; auto.
+  apply N.pow_nonzero.
+  discriminate.
+Qed.
+
+Theorem Forall_dest A (P : A -> Prop) x xs :
+  Forall P (x::xs) <-> P x /\ Forall P xs.
+  split; intro H; inversion H; auto.
+Qed.
+
+Theorem rv_encode_addi_check rd rs1 imm :
+  match rv_encode_addi rd rs1 imm with
+  | None => True
+  | Some (l,n) => l = 32 /\ rv_decode n = R5_Addi rd rs1 (scast 12 32 imm)
+  end.
+  unfold rv_encode_addi,rv_encode_i,rv_encodel_i,encode_be_bits,list2bv_opt.
+  simpl.
+  destruct bvl_valid_dec; auto.
+  split; auto.
+  unfold bvl_valid,bv_valid in b.
+  repeat rewrite Forall_dest in b.
+  simpl in b.
+  intuition.
+  unfold rv_decode.
+  repeat rewrite N.land_lor_distr_l.
+  repeat rewrite rv_shift_and_ones by discriminate; auto.
+  repeat rewrite N.lor_0_l.
+  simpl (19 .& _).
+  unfold rv_decode_op,xbits.
+  repeat rewrite N.shiftr_lor.
+  repeat rewrite N.shiftr_shiftl_l by discriminate.
+  repeat rewrite N.shiftr_shiftl_r by discriminate.
+  repeat rewrite N.shiftr_div_pow2.
+  repeat rewrite N.div_small by assumption.
+  repeat rewrite N.land_lor_distr_l.
+  repeat rewrite rv_shift_and_ones by discriminate.
+  repeat rewrite <- N.shiftr_div_pow2.
+  repeat rewrite N.land_0_l.
+  rewrite N.lor_0_r.
+  repeat rewrite N.shiftr_shiftl_l by discriminate.
+  repeat rewrite N.shiftr_shiftl_r by discriminate.
+  simpl (_ - _).
+  repeat rewrite N.shiftl_0_r.
+  repeat rewrite N.shiftr_0_r.
+  repeat rewrite rv_shift_and_ones by discriminate.
+  repeat rewrite N.shiftr_div_pow2.
+  fold (2^5) (2^7) (2^12) in *.
+  repeat rewrite N.div_small by
+      (eapply N.lt_le_trans,N.pow_le_mono_r; eauto; discriminate).
+  simpl.
+  repeat rewrite N.lor_0_r,N.land_ones.
+  repeat rewrite N.mod_small; auto.
+Qed.
+(* TODO: sign extension *)
+(* scast 12 32 (imm mod 2^32) == imm *)
+
+Definition rv_type :=
+  | R5_Lb : N -> N -> N -> rv_asm
+  | R5_Lh : N -> N -> N -> rv_asm
+  | R5_Lw : N -> N -> N -> rv_asm
+  | R5_Lbu : N -> N -> N -> rv_asm
+  | R5_Lhu : N -> N -> N -> rv_asm
+  | R5_Auipc : N -> N -> rv_asm
+  | R5_Sb : N -> N -> Z -> rv_asm
+  | R5_Sh : N -> N -> Z -> rv_asm
+  | R5_Sw : N -> N -> Z -> rv_asm
+  | R5_Add : N -> N -> N -> rv_asm
+  | R5_Sub : N -> N -> N -> rv_asm
+  | R5_Sll : N -> N -> N -> rv_asm
+  | R5_Slt : N -> N -> N -> rv_asm
+  | R5_Sltu : N -> N -> N -> rv_asm
+  | R5_Xor : N -> N -> N -> rv_asm
+  | R5_Srl : N -> N -> N -> rv_asm
+  | R5_Sra : N -> N -> N -> rv_asm
+  | R5_Or : N -> N -> N -> rv_asm
+  | R5_And : N -> N -> N -> rv_asm
+  | R5_Lui : N -> N -> rv_asm
+  | R5_Beq : N -> N -> Z -> rv_asm
+  | R5_Bne : N -> N -> Z -> rv_asm
+  | R5_Blt : N -> N -> Z -> rv_asm
+  | R5_Bge : N -> N -> Z -> rv_asm
+  | R5_Bltu : N -> N -> Z -> rv_asm
+  | R5_Bgeu : N -> N -> Z -> rv_asm
+  | R5_Jalr : N -> N -> Z -> rv_asm
+  | R5_Jal : N -> Z -> rv_asm
+  | R5_Addi : N -> N -> N -> rv_asm
+  | R5_Slli : N -> N -> N -> rv_asm
+  | R5_Slti : N -> N -> N -> rv_asm
+  | R5_Sltiu : N -> N -> N -> rv_asm
+  | R5_Xori : N -> N -> N -> rv_asm
+  | R5_Ori : N -> N -> N -> rv_asm
+  | R5_Andi : N -> N -> N -> rv_asm
+  | R5_Srli : N -> N -> N -> rv_asm
+  | R5_Srai : N -> N -> N -> rv_asm
+  | R5_Fence : N -> N -> rv_asm
+  | R5_Fence_i : rv_asm
+  | R5_InvalidI : rv_asm.
+
+Definition rv_encode :=
