cleanbyva2.v
@@ -1,0 +1,43 @@
+Require Import Picinae_armv7.
+Require Import NArith.
+Open Scope N.
+Open Scope stmt_scope.
+
+Definition cleanByVA : program := fun _ a => match a with
+
+(* 0xc0000034: ldr r0, [sp] *)
+| 0 => Some (4,
+    Move R_R0 (Load (Var V_MEM32) (Var R_SP) LittleE 4)
+  )
+
+(* 0xc0000038: mcr p15, #0x0, r0, c7, c10, #0x1 *)
+| 4 => Some (4,
+    Nop (* Special: unsupported: MCR *)
+  )
+
+(* 0xc000003c: mcr p15, #0x0, r0, c7, c10, #0x1 *)
+| 8 => Some (4,
+    Nop (* Special: unsupported: MCR *)
+  )
+
+(* 0xc0000040: dmb sy *)
+| 12 => Some (4,
+    Nop
+  )
+
+| _ => None
+end.
+
+Theorem cleanByVA_proof :
+  forall s m n w,
+  s V_MEM32 = VaM m w
+  -> s R_SP = VaN n w
+  -> (forall x, x < 4 -> mem_readable s (n + x))
+  -> exists s', exec_prog (fun _ => Some tt) cleanByVA 0 s 4 s' (Exit 16)
+                /\ forall v, v <> R_R0 -> s v = s' v.
+  intros.
+  eexists.
+  split; [|intros;rewrite update_frame;[reflexivity|eassumption]].
+  econstructor; [reflexivity|constructor|reflexivity|repeat econstructor].
+  econstructor; [rewrite <- H|rewrite <- H0|intuition]; econstructor.
+Qed.
