strtok_proofs.v
@@ -1,0 +1,103 @@
+Require Import Utf8.
+Require Import FunctionalExtensionality.
+Require Import Arith.
+Require Import NArith.
+Require Import ZArith.
+Require Import Picinae_i386.
+Require Import strtok_i386.
+Import List.
+
+Import X86Notations.
+
+Definition cstring m loc s :=
+  m Ⓑ[loc ⊕ N.of_nat (length s)] = 0 /\
+  ~In 0 s /\
+  forall n, (n < length s)%nat -> m Ⓑ[loc ⊕ N.of_nat n] = nth n s 0.
+
+Theorem cstringcdr m loc h t :
+  cstring m loc (cons h t) -> cstring m (loc + 1) t.
+  unfold cstring.
+  intuition; rewrite <- N.add_assoc,N.add_1_l,<- Nat2N.inj_succ; [assumption|].
+  apply H2.
+  simpl.
+  apply lt_n_S.
+  assumption.
+Qed.
+
+Theorem cstringcons m loc h t :
+  h <> 0
+  -> m Ⓑ[loc mod (2^32)] = h
+  -> cstring m (loc+1) t
+  -> cstring m loc (cons h t).
+  unfold cstring.
+  simpl (In _ _).
+  simpl length.
+  rewrite Nat2N.inj_succ,<- N.add_1_l,N.add_assoc.
+  intuition.
+  destruct n; [rewrite N.add_0_r;assumption|].
+  rewrite Nat2N.inj_succ,<- N.add_1_l,N.add_assoc.
+  simpl nth.
+  apply H4.
+  apply lt_S_n.
+  assumption.
+Qed.
+
+Definition strtok_charset m loc char := m Ⓑ[loc ⊕ char] <> 0.
+
+(* Definition strtok_post loc s s' := *)
+(*   exists m m' esp start startstr delim delimstr, *)
+(*     s V_MEM32 = Ⓜm -> *)
+(*     s R_ESP = Ⓓesp -> *)
+(*     s' V_MEM32 = Ⓜm' -> *)
+(*     cstring m start startstr -> *)
+(*     cstring m delim delimstr -> *)
+(*     (start = if (m Ⓓ[esp⊕4] =? 0) then m Ⓓ[loc] else m Ⓓ[esp⊕4]) /\ *)
+(*     if start =? 0 *)
+(*     then s' R_EAX = Ⓓ0 *)
+(*     else exists tok tokstr alld alldstr rest reststr result next, *)
+(*         cstring m tok tokstr /\ *)
+(*         cstring m alld alldstr /\ *)
+(*         cstring m rest reststr /\ *)
+(*         s' R_EAX = Ⓓresult /\ *)
+(*         m' Ⓓ[loc] = next /\ *)
+(*         cstring m' result tokstr /\ *)
+(*         startstr = tokstr ++ alldstr ++ reststr /\ *)
+(*         (forall c, List.In c alldstr -> List.In c delimstr) /\ *)
+(*         match reststr with *)
+(*         | nil => next = 0 *)
+(*         | cons h _ => ~List.In h delimstr /\ cstring m' next reststr *)
+(*         end. *)
+
+Definition strtok_post loc m strarg delim (_:exit) s' :=
+  exists m' delimstr,
+    s' V_MEM32 = Ⓜm' ->
+    cstring m delim delimstr ->
+    let start := if strarg =? 0 then m Ⓓ[loc] else strarg in
+    if start =? 0
+    then s' R_EAX = Ⓓ0
+    else exists startstr tok tokstr alld alldstr rest reststr,
+        cstring m start startstr /\
+        cstring m' tok tokstr /\
+        cstring m alld alldstr /\
+        cstring m rest reststr /\
+        s' R_EAX = Ⓓtok /\
+        startstr = tokstr ++ alldstr ++ reststr /\
+        (forall c, List.In c delimstr -> ~List.In c tokstr) /\
+        (forall c, List.In c alldstr -> List.In c delimstr) /\
+        match reststr with
+        | nil => m' Ⓓ[loc] = 0
+        | cons h _ => ~List.In h delimstr /\ cstring m' (m' Ⓓ[loc]) reststr
+        end.
+
+Definition strtok_invs loc morig strarg string delim delimstr a s :=
+  let args_inv :=
+      vmem (s V_MEM32) = 
+  let charset_inv :=
+      forall c,
+        List.In c delimstr
+        -> strtok_charset (vmem (s V_MEM32)) (vnum (s R_ESP)) c
+  in
+  match a with
+  | 18 =>
+    s R_EAX = None
+  end.
